src/smtencoding/FStar.SMTEncoding.Encode.fs
@@ -483,7 +483,8 @@ let is_BitVector_primitive head args =
       || S.fv_eq_lid fv Const.bv_shift_left_lid
       || S.fv_eq_lid fv Const.bv_shift_right_lid
       || S.fv_eq_lid fv Const.bv_udiv_lid
-      || S.fv_eq_lid fv Const.bv_mod_lid) &&
+      || S.fv_eq_lid fv Const.bv_mod_lid
+      || S.fv_eq_lid fv Const.bv_mul_lid) &&
       (isInteger sz_arg.n)
     | Tm_fvar fv, [(sz_arg, _); _] ->
         (S.fv_eq_lid fv Const.nat_to_bv_lid) &&
@@ -633,6 +634,7 @@ and encode_arith_term env head args_e =
     let bv_shr  = mk_bv (Util.mkBvShr sz) binary_arith in
     let bv_udiv = mk_bv (Util.mkBvUdiv sz) binary_arith in
     let bv_mod  = mk_bv (Util.mkBvMod sz) binary_arith in
+    let bv_mul  = mk_bv (Util.mkBvMul sz) binary_arith in
     let bv_to   = mk_bv (Util.mkNatToBv sz) unary_arith in
     let ops =
         [(Const.bv_and_lid, bv_and);
@@ -642,6 +644,7 @@ and encode_arith_term env head args_e =
          (Const.bv_shift_right_lid, bv_shr);
          (Const.bv_udiv_lid, bv_udiv);
          (Const.bv_mod_lid, bv_mod);
+         (Const.bv_mul_lid, bv_mul);
          (Const.nat_to_bv_lid, bv_to)]
     in
     let _, op =
