src/smtencoding/FStar.SMTEncoding.Util.fs
@@ -57,6 +57,7 @@ let mkBvShl sz = norng (mkBvShl sz)
 let mkBvShr sz = norng (mkBvShr sz)
 let mkBvUdiv sz = norng (mkBvUdiv sz)
 let mkBvMod sz = norng (mkBvMod sz)
+let mkBvMul sz = norng (mkBvMul sz)
 let mkITE = norng mkITE
 let mkCases = norng mkCases
 let mkForall = norng mkForall
